Refactor

src/Iris/Std/CoPset.lean
@@ -1,7 +1,8 @@
 import Iris.Std.Positives
+import Iris.Std.Classes
 
-/- This file implements an abstract type [coPset] of (possibly infinite) sets
-of positive binary natural numbers ([positive]). This type supports the
+/- This file implements an abstract type [CoPset] of (possibly infinite) sets
+of positive binary natural numbers ([Pos]). This type supports the
 following operations:
 
 · the empty set;
@@ -55,62 +56,61 @@ def CoPsetRaw.node' (b : Bool) (l r : CoPsetRaw) : CoPsetRaw :=
 
 theorem node'_wf b l r :
   coPset_wf l -> coPset_wf r -> coPset_wf (CoPsetRaw.node' b l r) := by
-  cases b <;> rcases l with ⟨ ⟨⟩ ⟩ | _ <;> rcases r with ⟨ ⟨⟩ ⟩ | _ <;> simp [CoPsetRaw.node', coPset_wf]
-  · exact fun a_6 a_7 => ⟨a_6, a_7⟩
-  · exact fun a_6 a_7 => ⟨a_6, a_7⟩
+  cases b <;> rcases l with ⟨ ⟨⟩ ⟩ | _ <;> rcases r with ⟨ ⟨⟩ ⟩ | _ <;>
+  simp [CoPsetRaw.node', coPset_wf] <;> exact fun a_6 a_7 => ⟨a_6, a_7⟩
 
 open CoPsetRaw
 
 /-- The membership test. -/
-def coPsetElemOfRaw : Pos → CoPsetRaw → Bool
+def CoPsetRaw.ElemOf : Pos → CoPsetRaw → Bool
   | _, leaf b => b
   | P1, node b _ _ => b
-  | p~0, node _ l _ => coPsetElemOfRaw p l
-  | p~1, node _ _ r => coPsetElemOfRaw p r
+  | p~0, node _ l _ => CoPsetRaw.ElemOf p l
+  | p~1, node _ _ r => CoPsetRaw.ElemOf p r
 instance : Membership Pos CoPsetRaw  where
-  mem := fun t p => coPsetElemOfRaw p t
+  mem := fun t p => CoPsetRaw.ElemOf p t
 
 theorem elem_of_node b l r (p : Pos) :
-  (coPsetElemOfRaw p (CoPsetRaw.node' b l r)) = (coPsetElemOfRaw p (CoPsetRaw.node b l r)) := by
+  (CoPsetRaw.ElemOf p (CoPsetRaw.node' b l r)) = (CoPsetRaw.ElemOf p (CoPsetRaw.node b l r)) := by
   cases p <;> cases b <;> rcases l with ⟨⟨⟩⟩ | _ <;> rcases r with ⟨⟨⟩⟩ | _ <;>
-  simp [node', coPsetElemOfRaw]
+  simp [node', CoPsetRaw.ElemOf]
 
 
 /-- Singleton. -/
-def coPsetSingletonRaw : Pos → CoPsetRaw
+def CoPsetRaw.Singleton : Pos → CoPsetRaw
   | P1 => node true (leaf false) (leaf false)
-  | p~0 => node' false (coPsetSingletonRaw p) (leaf false)
-  | p~1 => node' false (leaf false) (coPsetSingletonRaw p)
+  | p~0 => node' false (Singleton p) (leaf false)
+  | p~1 => node' false (leaf false) (Singleton p)
 
 /-- Union -/
-def coPsetUnionRaw : CoPsetRaw → CoPsetRaw → CoPsetRaw
+def CoPsetRaw.Union : CoPsetRaw → CoPsetRaw → CoPsetRaw
   | leaf false, t => t
   | t, leaf false => t
   | leaf true, _ => leaf true
   | _, leaf true => leaf true
   | node b1 l1 r1, node b2 l2 r2 =>
-    node' (b1 || b2) (coPsetUnionRaw l1 l2) (coPsetUnionRaw r1 r2)
-instance : Union CoPsetRaw where union := coPsetUnionRaw
+    node' (b1 || b2) (Union l1 l2) (Union r1 r2)
+instance : Union CoPsetRaw where union := CoPsetRaw.Union
 
 /-- Intersection -/
-def coPsetIntersectionRaw : CoPsetRaw → CoPsetRaw → CoPsetRaw
+def CoPsetRaw.Intersection : CoPsetRaw → CoPsetRaw → CoPsetRaw
   | leaf true, t => t
   | t, leaf true => t
   | leaf false, _ => leaf false
   | _, leaf false => leaf false
   | node b1 l1 r1, node b2 l2 r2 =>
-    node' (b1 && b2) (coPsetIntersectionRaw l1 l2) (coPsetIntersectionRaw r1 r2)
-instance : Inter CoPsetRaw where inter := coPsetIntersectionRaw
+    node' (b1 && b2) (Intersection l1 l2) (Intersection r1 r2)
+instance : Inter CoPsetRaw where inter := CoPsetRaw.Intersection
 
 /-- Complement -/
-def coPsetComplementRaw : CoPsetRaw → CoPsetRaw
+def CoPsetRaw.Complement : CoPsetRaw → CoPsetRaw
   | leaf b => leaf (!b)
-  | node b l r => node' (!b) (coPsetComplementRaw l) (coPsetComplementRaw r)
+  | node b l r => node' (!b) (Complement l) (Complement r)
 
 /-- Well-formedness for the above operations -/
 
-theorem coPsetSingleton_wf p : coPset_wf (coPsetSingletonRaw p) := by
-  induction p <;> simp_all [coPsetSingletonRaw, coPset_wf]
+theorem coPsetSingleton_wf p : coPset_wf (CoPsetRaw.Singleton p) := by
+  induction p <;> simp_all [CoPsetRaw.Singleton, coPset_wf]
   · apply node'_wf; simp [coPset_wf]; assumption
   · apply node'_wf; assumption; simp [coPset_wf]
 
@@ -118,11 +118,11 @@ theorem coPsetUnion_wf t1 t2 :
   coPset_wf t1 -> coPset_wf t2 -> coPset_wf (t1 ∪ t2) := by
   revert t2; induction t1 with
   | leaf b =>
-    intros t2 Hwf1 Hwf2; cases b <;> simp [Union.union, coPsetUnionRaw]
+    intros t2 Hwf1 Hwf2; cases b <;> simp [Union.union, CoPsetRaw.Union]
     · assumption
-    · rcases t2 with ⟨⟨⟩⟩ | _ <;> simp [coPsetUnionRaw, coPset_wf]
+    · rcases t2 with ⟨⟨⟩⟩ | _ <;> simp [CoPsetRaw.Union, coPset_wf]
   | node b l r IH1 IH2 =>
-    intros t2 Hwf1 Hwf2; rcases t2 with ⟨⟨⟩⟩ | _ <;> simp [Union.union, coPsetUnionRaw, coPset_wf]
+    intros t2 Hwf1 Hwf2; rcases t2 with ⟨⟨⟩⟩ | _ <;> simp [Union.union, CoPsetRaw.Union, coPset_wf]
     · assumption
     · apply node'_wf
       · apply IH1; exact node_wf_l b l r Hwf1
@@ -134,11 +134,11 @@ theorem coPsetIntersection_wf t1 t2 :
   coPset_wf t1 -> coPset_wf t2 -> coPset_wf (t1 ∩ t2) := by
   revert t2; induction t1 with
   | leaf b =>
-    intros t2 Hwf1 Hwf2; cases b <;> simp [Inter.inter, coPsetIntersectionRaw]
-    · rcases t2 with ⟨⟨⟩⟩ | _ <;> simp [coPsetIntersectionRaw, coPset_wf]
+    intros t2 Hwf1 Hwf2; cases b <;> simp [Inter.inter, CoPsetRaw.Intersection]
+    · rcases t2 with ⟨⟨⟩⟩ | _ <;> simp [CoPsetRaw.Intersection, coPset_wf]
     · assumption
   | node b l r IH1 IH2 =>
-    intros t2 Hwf1 Hwf2; rcases t2 with ⟨⟨⟩⟩ | _ <;> simp [Inter.inter, coPsetIntersectionRaw, coPset_wf]
+    intros t2 Hwf1 Hwf2; rcases t2 with ⟨⟨⟩⟩ | _ <;> simp [Inter.inter, CoPsetRaw.Intersection, coPset_wf]
     · assumption
     · apply node'_wf
       · apply IH1; exact node_wf_l b l r Hwf1
@@ -146,10 +146,10 @@ theorem coPsetIntersection_wf t1 t2 :
       · apply IH2; exact node_wf_r b l r Hwf1
         (expose_names; exact node_wf_r a a_1 a_2 Hwf2)
 
-theorem coPsetComplement_wf t : coPset_wf (coPsetComplementRaw t) := by
+theorem coPsetComplement_wf t : coPset_wf (CoPsetRaw.Complement t) := by
   induction t with
-  | leaf b => cases b <;> simp [coPsetComplementRaw, coPset_wf]
-  | node b l r => cases b <;> simp [coPsetComplementRaw, coPset_wf] <;>
+  | leaf b => cases b <;> simp [CoPsetRaw.Complement, coPset_wf]
+  | node b l r => cases b <;> simp [CoPsetRaw.Complement, coPset_wf] <;>
     apply node'_wf <;> assumption
 
 /-- The abstract type [CoPset] -/
@@ -170,24 +170,24 @@ instance : EmptyCollection CoPset where emptyCollection := CoPset.empty
 def full : CoPset := ⟨CoPsetRaw.leaf true, rfl⟩
 
 def singleton (p : Pos) : CoPset :=
-  ⟨coPsetSingletonRaw p, coPsetSingleton_wf p⟩
+  ⟨CoPsetRaw.Singleton p, coPsetSingleton_wf p⟩
 
 def union (X Y : CoPset) : CoPset :=
-  ⟨coPsetUnionRaw X.tree Y.tree, coPsetUnion_wf _ _ X.wf Y.wf⟩
+  ⟨CoPsetRaw.Union X.tree Y.tree, coPsetUnion_wf _ _ X.wf Y.wf⟩
 instance : Union CoPset where union := CoPset.union
 
 def inter (X Y : CoPset) : CoPset :=
-  ⟨coPsetIntersectionRaw X.tree Y.tree, coPsetIntersection_wf _ _ X.wf Y.wf⟩
+  ⟨CoPsetRaw.Intersection X.tree Y.tree, coPsetIntersection_wf _ _ X.wf Y.wf⟩
 instance : Inter CoPset where inter := CoPset.inter
 
 def diff (X Y : CoPset) : CoPset :=
-  ⟨coPsetIntersectionRaw X.tree (coPsetComplementRaw Y.tree), coPsetIntersection_wf _ _ X.wf (coPsetComplement_wf _)⟩
+  ⟨CoPsetRaw.Intersection X.tree (CoPsetRaw.Complement Y.tree), coPsetIntersection_wf _ _ X.wf (coPsetComplement_wf _)⟩
 
 def mem (p : Pos) (X : CoPset) : Bool :=
-  coPsetElemOfRaw p X.tree
+  CoPsetRaw.ElemOf p X.tree
 
 def complement (X : CoPset) : CoPset :=
-  ⟨coPsetComplementRaw X.tree, coPsetComplement_wf _⟩
+  ⟨CoPsetRaw.Complement X.tree, coPsetComplement_wf _⟩
 
 instance : HasSubset CoPset where
   Subset t1 t2 := ∀ (p : Pos), p ∈ t1 -> p ∈ t2
@@ -199,12 +199,12 @@ theorem subseteq_trans (X Y Z : CoPset) :
   intros Hxy Hyz p Hx
   exact Hyz p (Hxy p Hx)
 
-def isFiniteRaw : CoPsetRaw → Bool
+def CoPsetRaw.isFinite : CoPsetRaw → Bool
   | CoPsetRaw.leaf b => !b
-  | CoPsetRaw.node _ l r => isFiniteRaw l && isFiniteRaw r
+  | CoPsetRaw.node _ l r => isFinite l && isFinite r
 
 def isFinite (X : CoPset) : Bool :=
-  isFiniteRaw X.tree
+  CoPsetRaw.isFinite X.tree
 
 /-- Picking an element out of an infinite set -/
 
@@ -232,43 +232,43 @@ def CoPset.pick (X : CoPset) : Pos :=
 of [p], when these numbers are viewed as sequences of bits. In other words, it
 is the set of all numbers that have the suffix [q]. It is always an infinite
 set. -/
-def suffixesRaw : Pos → CoPsetRaw
+def CoPsetRaw.suffixesRaw : Pos → CoPsetRaw
   | P1 => .leaf true
   | p~0 => CoPsetRaw.node' false (suffixesRaw p) (.leaf false)
   | p~1 => CoPsetRaw.node' false (.leaf false) (suffixesRaw p)
 
-theorem coPsetSuffixes_wf p : coPset_wf (suffixesRaw p) := by
-  induction p <;> simp [suffixesRaw, coPset_wf] <;>
+theorem coPsetSuffixes_wf p : coPset_wf (CoPsetRaw.suffixesRaw p) := by
+  induction p <;> simp [CoPsetRaw.suffixesRaw, coPset_wf] <;>
   apply node'_wf <;> simp_all [coPset_wf]
 
 def suffixes (p : Pos) : CoPset :=
-  ⟨suffixesRaw p, coPsetSuffixes_wf p⟩
+  ⟨CoPsetRaw.suffixesRaw p, coPsetSuffixes_wf p⟩
 theorem elem_suffixes p q : p ∈ suffixes q <-> ∃ q', p = q' ++ q := by
   constructor
   · induction q generalizing p with
     | xI q IH =>
-      simp [suffixes, suffixesRaw]
+      simp [suffixes, CoPsetRaw.suffixesRaw]
       simp_all [Membership.mem]; rewrite [elem_of_node]
-      intros Hin; cases p <;> simp [coPsetElemOfRaw] at Hin
+      intros Hin; cases p <;> simp [CoPsetRaw.ElemOf] at Hin
       specialize (IH _ Hin)
       rcases IH with ⟨ q', Heq ⟩
       exists q'; rewrite [Heq]; simp [HAppend.hAppend, Pos.app]
     | xO q IH =>
-      simp [suffixes, suffixesRaw]
+      simp [suffixes, CoPsetRaw.suffixesRaw]
       simp_all [Membership.mem]; rewrite [elem_of_node]
-      intros Hin; cases p <;> simp [coPsetElemOfRaw] at Hin
+      intros Hin; cases p <;> simp [CoPsetRaw.ElemOf] at Hin
       specialize (IH _ Hin)
       rcases IH with ⟨ q', Heq ⟩
       exists q'; rewrite [Heq]; simp [HAppend.hAppend, Pos.app]
     | xH =>
-      simp [suffixes, suffixesRaw]
-      simp [Membership.mem, coPsetElemOfRaw]
+      simp [suffixes, CoPsetRaw.suffixesRaw]
+      simp [Membership.mem, CoPsetRaw.ElemOf]
       simp [HAppend.hAppend, Pos.app]
   · intros Heq; rcases Heq with ⟨ q', Heq ⟩; rewrite [Heq]
     simp [suffixes, Membership.mem]
-    induction q generalizing p <;> simp [suffixesRaw] <;> try rewrite [elem_of_node] <;>
-    simp_all [HAppend.hAppend, Pos.app, coPsetElemOfRaw]
-    cases q' <;> simp [coPsetElemOfRaw]
+    induction q generalizing p <;> simp [CoPsetRaw.suffixesRaw] <;> try rewrite [elem_of_node] <;>
+    simp_all [HAppend.hAppend, Pos.app, CoPsetRaw.ElemOf]
+    cases q' <;> simp [CoPsetRaw.ElemOf]
 
 /-- Splitting a set -/
 
@@ -307,12 +307,7 @@ def split (X : CoPset) : CoPset × CoPset :=
 
 end CoPset
 
-class Disjoint (α : Type u) where
-  disjoint : α -> α -> Prop
-
-infix:70 " ## " => Disjoint.disjoint
-
-instance : Disjoint CoPset where
+instance : Iris.Std.Disjoint CoPset where
   disjoint s t := ∀ p, p ∈ s -> p ∈ t -> False
 
 @[symm]
